02Typed/Typechecking.thy
@@ -341,35 +341,6 @@ proof -
   ultimately show "Map.empty \<turnstile>\<^sub>n e\<^sub>t : t" by simp
 qed
 
-lemma [simp]: "typecheck' \<Gamma> vs e = (e', t, vs', con) \<Longrightarrow> 
-  valid_ty_subst \<Gamma> \<Longrightarrow> unify' con = Some sub' \<Longrightarrow> 
-    map_option (typeify \<circ> subst sub) \<circ> \<Gamma> \<turnstile>\<^sub>n solidify (hsubst sub e') : typeify (subst sub t) \<Longrightarrow>
-      sub extends sub'"
-proof (induction arbitrary: sub' rule: typecheck_induct)
-  case (NLam \<Gamma> vs vs' con x e\<^sub>1 e\<^sub>1' t' v)
-  moreover hence "map_option (typeify \<circ> subst sub) \<circ> \<Gamma> \<turnstile>\<^sub>n 
-    solidify (hsubst sub (HLam x (Var v) e\<^sub>1')) : typeify (subst sub (Ctor ''Arrow'' [Var v, t']))" 
-      by blast
-  ultimately show ?case by fastforce
-next
-  case (NApp \<Gamma> vs vs' e\<^sub>1 e\<^sub>2 v e\<^sub>1' t\<^sub>1 vs'' con\<^sub>1 e\<^sub>2' t\<^sub>2 con\<^sub>2)
-  from NApp have "v = fresh vs" by simp
-  from NApp have "typecheck' \<Gamma> (insert v vs) e\<^sub>1 = (e\<^sub>1', t\<^sub>1, vs'', con\<^sub>1)" by simp
-  from NApp have "typecheck' \<Gamma> vs'' e\<^sub>2 = (e\<^sub>2', t\<^sub>2, vs', con\<^sub>2)" by simp
-  from NApp have "unify' con\<^sub>1 = Some xsub' \<Longrightarrow>
-    map_option (typeify \<circ> subst sub) \<circ> \<Gamma> \<turnstile>\<^sub>n solidify (hsubst sub e\<^sub>1') : typeify (subst sub t\<^sub>1) \<Longrightarrow> sub extends xsub'" by blast
-  from NApp have "unify' con\<^sub>2 = Some xsub' \<Longrightarrow>
-    map_option (typeify \<circ> subst sub) \<circ> \<Gamma> \<turnstile>\<^sub>n solidify (hsubst sub e\<^sub>2') : typeify (subst sub t\<^sub>2) \<Longrightarrow> sub extends xsub'" by blast
-  from NApp have "valid_ty_subst \<Gamma>" by simp
-  from NApp have "unify' (con\<^sub>1 @ con\<^sub>2 @ [(t\<^sub>1, Ctor ''Arrow'' [t\<^sub>2, Var v])]) = Some sub'" by simp
-  from NApp have "map_option (typeify \<circ> subst sub) \<circ> \<Gamma> \<turnstile>\<^sub>n solidify (hsubst sub (HApp e\<^sub>1' e\<^sub>2')) : typeify (subst sub (Var v))" by blast
-
-
-
-  have "sub extends sub'" by simp
-  thus ?case by simp
-qed auto
-
 lemma [simp]: "typecheck' \<Gamma> vs e = (e', t, vs', con) \<Longrightarrow> e = erase (solidify e')"
   by (induction rule: typecheck_induct) auto
 
@@ -528,8 +499,8 @@ proof (induction "map_option typeify \<circ> \<Gamma>" e\<^sub>t t arbitrary: \<
 next
   case (tcn_app e\<^sub>1 t\<^sub>1 t\<^sub>2 e\<^sub>2)
   let ?v = "fresh vs"
-  obtain e\<^sub>1' tt\<^sub>1 vs'' con\<^sub>1 where T1: "typecheck' \<Gamma> (extend_set vs) (erase e\<^sub>1) = (e\<^sub>1', tt\<^sub>1, vs'', con\<^sub>1)"
-    by (metis prod_cases4)
+  obtain e\<^sub>1' tt\<^sub>1 vs'' con\<^sub>1 where T1: "typecheck' \<Gamma> (extend_set vs) (erase e\<^sub>1) = 
+    (e\<^sub>1', tt\<^sub>1, vs'', con\<^sub>1)" by (metis prod_cases4)
   obtain e\<^sub>2' tt\<^sub>2 vs''' con\<^sub>2 where T2: "typecheck' \<Gamma> vs'' (erase e\<^sub>2) = (e\<^sub>2', tt\<^sub>2, vs''', con\<^sub>2)"
     by (metis prod_cases4)
   from tcn_app T1 T2 have E: "e' = HApp e\<^sub>1' e\<^sub>2' \<and> tt = Var ?v \<and> vs''' = vs' \<and> 
@@ -541,14 +512,12 @@ next
 
 
   from tcn_app have "tvarst e\<^sub>1 \<subseteq> extend_set vs" by auto
-  with tcn_app T1 obtain s\<^sub>1 where "unify' con\<^sub>1 = Some s\<^sub>1" by blast
+  with tcn_app T1 obtain s\<^sub>1 where S1: "unify' con\<^sub>1 = Some s\<^sub>1" by blast
   with tcn_app T1 have "sub extends s\<^sub>1 \<Longrightarrow>
     map_option (typeify \<circ> subst sub) \<circ> \<Gamma> \<turnstile>\<^sub>n solidify (hsubst sub e\<^sub>1') : typeify (subst sub tt\<^sub>1)" 
       by (metis typecheck_succeeds)
   with tcn_app VH VT have "sub extends s\<^sub>1 \<Longrightarrow> map_option (tsubsts sub) \<circ> map_option typeify \<circ> \<Gamma> \<turnstile>\<^sub>n 
     tsubstt sub (solidify e\<^sub>1') : tsubsts sub (typeify tt\<^sub>1)" by simp
-
-  from tcn_app have "map_option typeify \<circ> \<Gamma> \<turnstile>\<^sub>n e\<^sub>1 : Arrow t\<^sub>1 t\<^sub>2" by simp
 
 
   from T1 have "extend_set vs \<subseteq> vs''" by (metis vars_expand)
@@ -560,15 +529,31 @@ next
 
 
 
+  from tcn_app have "map_option typeify \<circ> \<Gamma> \<turnstile>\<^sub>n e\<^sub>1 : Arrow t\<^sub>1 t\<^sub>2" by simp
   from tcn_app have "map_option typeify \<circ> \<Gamma> \<turnstile>\<^sub>n e\<^sub>2 : t\<^sub>1" by simp
   from tcn_app have "finite vs" by simp
   from tcn_app have "subst_vars \<Gamma> \<subseteq> vs" by simp
-  from tcn_app have "tvarst (TApp e\<^sub>1 e\<^sub>2) \<subseteq> vs" by simp
+  from tcn_app have "tvarst e\<^sub>1 \<subseteq> vs" by simp
+  from tcn_app have "tvarst e\<^sub>2 \<subseteq> vs" by simp
   from tcn_app have "valid_ty_subst \<Gamma>" by simp
 
+  from tcn_app have "?v \<notin> subst_vars \<Gamma>" by auto
+  with tcn_app T1 have "?v \<notin> list_vars con\<^sub>1" by simp
+  with S1 have "?v \<notin> dom s\<^sub>1" using unify_dom by blast 
+  hence V: "s\<^sub>1 ?v = None" by auto
 
-  from tcn_app E have "unify' (con\<^sub>1 @ con\<^sub>2 @ [(tt\<^sub>1, Ctor ''Arrow'' [tt\<^sub>2, Var ?v])]) = None" by simp
 
+
+  from tcn_app E have "unify' (con\<^sub>1 @ (con\<^sub>2 @ [(tt\<^sub>1, Ctor ''Arrow'' [tt\<^sub>2, Var ?v])])) = None" by simp
+  hence "unify' con\<^sub>1 = None \<or> (\<exists>s. unify' con\<^sub>1 = Some s \<and> 
+    unify' (map (pair_subst s) (con\<^sub>2 @ [(tt\<^sub>1, Ctor ''Arrow'' [tt\<^sub>2, Var ?v])])) = None)" 
+      by (metis unify_append_none)
+  with S1 V have "unify' (map (pair_subst s\<^sub>1) con\<^sub>2 @ 
+    [(subst s\<^sub>1 tt\<^sub>1, Ctor ''Arrow'' [subst s\<^sub>1 tt\<^sub>2, Var ?v])]) = None" by simp
+  hence "unify' (map (pair_subst s\<^sub>1) con\<^sub>2) = None \<or> 
+    (\<exists>s. unify' (map (pair_subst s\<^sub>1) con\<^sub>2) = Some s \<and> 
+      unify' (map (pair_subst s) [(subst s\<^sub>1 tt\<^sub>1, Ctor ''Arrow'' [subst s\<^sub>1 tt\<^sub>2, Var ?v])]) = None)" 
+        by (metis unify_append_none)
 
 
   have False by simp
